test/SumMaxLen.v
@@ -1,0 +1,281 @@
+(******************************************************************************)
+(* Copyright (c) 2022 Steven Keuchel                                          *)
+(* All rights reserved.                                                       *)
+(*                                                                            *)
+(* Redistribution and use in source and binary forms, with or without         *)
+(* modification, are permitted provided that the following conditions are     *)
+(* met:                                                                       *)
+(*                                                                            *)
+(* 1. Redistributions of source code must retain the above copyright notice,  *)
+(*    this list of conditions and the following disclaimer.                   *)
+(*                                                                            *)
+(* 2. Redistributions in binary form must reproduce the above copyright       *)
+(*    notice, this list of conditions and the following disclaimer in the     *)
+(*    documentation and/or other materials provided with the distribution.    *)
+(*                                                                            *)
+(* THIS SOFTWARE IS PROVIDED BY THE COPYRIGHT HOLDERS AND CONTRIBUTORS        *)
+(* "AS IS" AND ANY EXPRESS OR IMPLIED WARRANTIES, INCLUDING, BUT NOT LIMITED  *)
+(* TO, THE IMPLIED WARRANTIES OF MERCHANTABILITY AND FITNESS FOR A PARTICULAR *)
+(* PURPOSE ARE DISCLAIMED. IN NO EVENT SHALL THE COPYRIGHT HOLDER OR          *)
+(* CONTRIBUTORS BE LIABLE FOR ANY DIRECT, INDIRECT, INCIDENTAL, SPECIAL,      *)
+(* EXEMPLARY, OR CONSEQUENTIAL DAMAGES (INCLUDING, BUT NOT LIMITED TO,        *)
+(* PROCUREMENT OF SUBSTITUTE GOODS OR SERVICES; LOSS OF USE, DATA, OR         *)
+(* PROFITS; OR BUSINESS INTERRUPTION) HOWEVER CAUSED AND ON ANY THEORY OF     *)
+(* LIABILITY, WHETHER IN CONTRACT, STRICT LIABILITY, OR TORT (INCLUDING       *)
+(* NEGLIGENCE OR OTHERWISE) ARISING IN ANY WAY OUT OF THE USE OF THIS         *)
+(* SOFTWARE, EVEN IF ADVISED OF THE POSSIBILITY OF SUCH DAMAGE.               *)
+(******************************************************************************)
+
+From Coq Require Import
+     Lists.List
+     Logic.FinFun
+     Program.Tactics
+     Strings.String
+     ZArith.ZArith
+     micromega.Lia.
+
+From Equations Require Import
+     Equations.
+
+From Katamaran Require Import
+     Semantics.Registers
+     Shallow.Executor
+     Symbolic.Mutator
+     Symbolic.Solver
+     Symbolic.Worlds
+     Symbolic.Propositions
+     Specification
+     Program
+     Syntax.Predicates
+     Syntax.ContractDecl.
+
+Set Implicit Arguments.
+Import ctx.notations.
+Import env.notations.
+Open Scope string_scope.
+Open Scope Z_scope.
+Open Scope ctx_scope.
+
+(*** PROGRAM ***)
+
+Import DefaultBase.
+
+Module Import ExampleProgram <: Program DefaultBase.
+
+  Section FunDeclKit.
+
+    Inductive Fun : PCtx -> Ty -> Set :=
+    | summaxlen : Fun [ "xs" ∷ ty.list ty.int ] (ty.prod (ty.prod ty.int ty.int) ty.int)
+    .
+
+    Definition 𝑭  : PCtx -> Ty -> Set := Fun.
+    Definition 𝑭𝑿 : PCtx -> Ty -> Set := fun _ _ => Empty_set.
+    Definition 𝑳 : PCtx -> Set := fun _ => Empty_set.
+
+  End FunDeclKit.
+
+  Include FunDeclMixin DefaultBase.
+
+  Section FunDefKit.
+    Import ctx.resolution.
+
+    Local Coercion stm_exp : Exp >-> Stm.
+    Local Notation "'l'"   := (@exp_var _ "l" _ _) : exp_scope.
+    Local Notation "'m'"   := (@exp_var _ "m" _ _) : exp_scope.
+    Local Notation "'s'"   := (@exp_var _ "s" _ _) : exp_scope.
+    Local Notation "'sm'"   := (@exp_var _ "sm" _ _) : exp_scope.
+    Local Notation "'sml'"   := (@exp_var _ "sml" _ _) : exp_scope.
+    Local Notation "'y'"   := (@exp_var _ "y" _ _) : exp_scope.
+    Local Notation "'xs'"   := (@exp_var _ "xs" _ _) : exp_scope.
+    Local Notation "'ys'"   := (@exp_var _ "ys" _ _) : exp_scope.
+
+    Definition fun_summaxlen : Stm ["xs" ∷ ty.list ty.int] (ty.prod (ty.prod ty.int ty.int) ty.int) :=
+      stm_match_list xs (stm_val (ty.prod (ty.prod ty.int ty.int) ty.int) (0,0,0))
+        "y" "ys"
+        (let: "sml" := call summaxlen ys in
+         match: sml in (ty.prod ty.int ty.int , ty.int) with
+         | ("sm","l") =>
+           match: sm in (ty.int,ty.int) with
+           | ("s","m") =>
+             let: "m'" := if: m < y then y else m in
+             exp_binop bop.pair (exp_binop bop.pair (s + y) (exp_var "m'")) (l + exp_int 1)
+           end
+         end).
+
+    Definition fun_summaxlen_with_debug : Stm ["xs" ∷ ty.list ty.int] (ty.prod (ty.prod ty.int ty.int) ty.int) :=
+      stm_match_list xs (stm_val (ty.prod (ty.prod ty.int ty.int) ty.int) (0,0,0))
+        "y" "ys"
+        (let: "sml" := call summaxlen ys in
+         match: sml in (ty.prod ty.int ty.int , ty.int) with
+         | ("sm","l") =>
+             match: sm in (ty.int,ty.int) with
+             | ("s","m") =>
+                 let: "m'" := if: m < y then y else m in
+                 stm_debugk (exp_binop bop.pair (exp_binop bop.pair (s + y) (exp_var "m'")) (l + exp_int 1))
+             end
+         end).
+
+    Definition FunDef {Δ τ} (f : Fun Δ τ) : Stm Δ τ :=
+      match f in Fun Δ τ return Stm Δ τ with
+      | summaxlen => fun_summaxlen
+      end.
+
+  End FunDefKit.
+
+  Include DefaultRegStoreKit DefaultBase.
+
+  Section ForeignKit.
+    Definition Memory : Set := unit.
+    Definition ForeignCall {σs σ} (f : 𝑭𝑿 σs σ) (args : NamedEnv Val σs)
+      (res : string + Val σ) (γ γ' : RegStore) (μ μ' : Memory) : Prop := False.
+    Lemma ForeignProgress {σs σ} (f : 𝑭𝑿 σs σ) (args : NamedEnv Val σs) γ μ :
+      exists γ' μ' res, ForeignCall f args res γ γ' μ μ'.
+    Proof. destruct f. Qed.
+  End ForeignKit.
+
+  Include ProgramMixin DefaultBase.
+
+End ExampleProgram.
+
+Module Import ExampleSig <: ProgramLogicSignature DefaultBase.
+  Module PROG := ExampleProgram.
+  Import ctx.resolution.
+
+  Include DefaultPredicateKit DefaultBase.
+  Include ContractDeclMixin DefaultBase ExampleProgram.
+  Include SpecificationMixin DefaultBase ExampleProgram.
+End ExampleSig.
+
+Module Import ExampleSpecification <: Specification DefaultBase ExampleSig.
+
+  Import ctx.resolution.
+
+  Definition sep_contract_summaxlen : SepContract [ "xs" ∷ ty.list ty.int ] (ty.prod (ty.prod ty.int ty.int) ty.int) :=
+    {| sep_contract_logic_variables := ["xs" ∷ ty.list ty.int ];
+       sep_contract_localstore      := [term_var "xs"];
+       sep_contract_precondition    := asn_true;
+       sep_contract_result          := "result";
+       sep_contract_postcondition   :=
+         asn_match_prod
+           (term_var "result") "sm" "l"
+           (asn_match_prod
+              (term_var "sm") "s" "m"
+              (asn_sep
+                 (asn_formula (formula_le (term_var "s") (term_binop bop.times (term_var "m") (term_var "l"))))
+                 (asn_formula (formula_le (term_val ty.int 0) (term_var "l")))));
+    |}.
+
+  Definition CEnv : SepContractEnv :=
+    fun Δ τ f =>
+      match f with
+      | summaxlen => Some sep_contract_summaxlen
+      end.
+
+  Definition CEnvEx : SepContractEnvEx :=
+    fun Δ τ f =>
+      match f with end.
+
+  Definition LEnv : LemmaEnv :=
+    fun Δ l =>
+      match l with end.
+
+End ExampleSpecification.
+
+Module ExampleSolverKit := DefaultSolverKit DefaultBase ExampleSig ExampleSpecification.
+Module ExampleSolver := MakeSolver DefaultBase ExampleSig ExampleSpecification ExampleSolverKit.
+
+Module Import ExampleExecutor :=
+  MakeExecutor DefaultBase ExampleSig ExampleSpecification ExampleSolver.
+
+Local Ltac solve :=
+  repeat
+    (repeat
+       match goal with
+       | H: _ /\ _ |- _ => destruct H
+       | H: Z.ltb _ _ = true |- _ => apply Z.ltb_lt in H
+       | H: Z.ltb _ _ = false |- _ => apply Z.ltb_ge in H
+       | H: pair _ _ = pair _ _ |- _ => inversion H; subst; clear H
+       | H: ?x = ?x |- _ => clear H
+       | |- forall _, _ => intro
+       | |- exists _, _ => eexists
+       | |- _ /\ _ => constructor
+       | |- _ = _  => reflexivity
+       end;
+     try progress subst);
+  auto.
+
+Module Import ExampleShalExec := MakeShallowExecutor DefaultBase ExampleSig ExampleSpecification.
+Import CMut.
+
+Goal True. idtac "Timing before: summaxlen/shallow". Abort.
+Lemma valid_contract_summaxlen_shallow : CMut.ValidContract 1 sep_contract_summaxlen fun_summaxlen.
+Proof.
+  compute - [negb Z.mul Z.opp Z.compare Z.add Z.geb Z.eqb Z.leb Z.gtb Z.ltb Z.le Z.lt Z.gt Z.ge].
+  solve; nia.
+Qed.
+Goal True. idtac "Timing after: summaxlen/shallow". Abort.
+
+(* Goal True. idtac "Timing before: summaxlen/slow". Abort. *)
+(* Lemma valid_contract_summaxlen_slow : SMut.ValidContract sep_contract_summaxlen fun_summaxlen. *)
+(* Proof. *)
+(*   compute. constructor. *)
+(*   compute - [Z.mul Z.add Z.le Z.ge Z.lt]. *)
+(*   solve; nia. *)
+(* Time Qed. *)
+(* Goal True. idtac "Timing after: summaxlen/slow". Abort. *)
+
+Goal True. idtac "Timing before: summaxlen/symbolic". Abort.
+Lemma valid_contract_summaxlen : SMut.ValidContract sep_contract_summaxlen fun_summaxlen.
+Proof.
+  apply SMut.validcontract_with_erasure_sound.
+  hnf.
+  compute. constructor.
+  compute - [Z.mul Z.add Z.le Z.ge Z.lt].
+  solve; nia.
+Qed.
+Goal True. idtac "Timing after: summaxlen/symbolic". Abort.
+
+Section Debug.
+
+  Goal CMut.ValidContract 1 sep_contract_summaxlen fun_summaxlen.
+    compute - [negb Z.mul Z.opp Z.compare Z.add Z.geb Z.eqb Z.leb Z.gtb Z.ltb Z.le Z.lt Z.gt Z.ge].
+    change
+      (forall xs : list Z, true = true ->
+         (nil = xs -> exists (sm : Z * Z) (l : Z), (sm,l) = (0, 0, 0) /\
+            (exists s m : Z, (s, m) = sm /\ s <= m * l /\ 0 <= l /\ True)) /\
+      (forall (y : Z) (ys : list Z), y :: ys = xs -> exists ys' : list Z, ys' = ys /\ true = true /\
+         (forall (sml : Z * Z * Z) (sm : Z * Z) (l : Z), (sm, l) = sml ->
+          forall s m : Z, (s, m) = sm -> s <= m * l -> 0 <= l ->
+          forall (sm' : Z * Z) (l' : Z), (sm', l') = sml -> forall s' m' : Z, (s',m') = sm' ->
+          ((m' <? y) = true -> exists (sm'' : Z * Z) (l'' : Z), (sm'', l'') = (s' + y, y, l' + 1) /\
+             (exists s'' m'' : Z, (s'', m'') = sm'' /\ s'' <= m'' * l'' /\ 0 <= l'' /\ True)) /\
+          ((m' <? y) = false -> exists (sm'' : Z * Z) (l'' : Z), (sm'', l'') = (s' + y, m', l' + 1) /\
+             (exists s'' m'' : Z, (s'', m'') = sm'' /\ s'' <= m'' * l'' /\ 0 <= l'' /\ True)))))%list.
+    idtac "Shallow verification condition:".
+    match goal with |- ?x => idtac x end.
+  Abort.
+
+  Import ty.
+  Import SymProp.
+  Import SymProp.notations.
+
+  Goal SMut.ValidContract sep_contract_summaxlen fun_summaxlen.
+    compute.
+    idtac "Symbolic verification condition:".
+    match goal with |- VerificationCondition ?x => idtac x end.
+  Abort.
+
+  Goal SMut.ValidContract sep_contract_summaxlen fun_summaxlen_with_debug.
+    compute.
+    idtac "Symbolic verification condition with debug nodes:".
+    match goal with |- VerificationCondition ?x => idtac x end.
+    idtac "Second debug node:".
+    match goal with
+    | |- context[SymProp.assumek
+                   (formula_ge _ _)
+                   (SymProp.debug (MkAMessage _ ?x) _)] =>
+        idtac x
+    end.
+  Abort.
+
+End Debug.
